run/eval for errS

coq/Util/ErrorWithState.v
@@ -4,50 +4,77 @@ Require Import ExtLib.Structures.Monads.
 Require Import ExtLib.Structures.Monad.
 Require Import ExtLib.Structures.MonadExc.
 Require Import ExtLib.Structures.MonadState.
-
 Require Import ExtLib.Data.Monads.EitherMonad.
 
+Require Import Vellvm.Error.
 
 Import MonadNotation.
 Open Scope monad_scope.
 Open Scope type_scope.
 
-Definition errS St A := St -> string+(St*A).
+Section withState.
 
-Instance Monad_errS St: Monad (errS St) :=
-  { ret  := fun _ x => fun s => inr (s,x)
-    ; bind := fun _ _ m f => fun s => match m s with
-                                | inl v => inl v
-                                | inr (s',x) => f x s'
-                                end
-  }.
+  Variable St : Type.
+  
+  Definition errS A := St -> string+(St*A).
 
-Instance Exception_errS St : MonadExc string (errS St) :=
-  { raise := fun _ v => fun s => inl v
-    ; catch := fun _ c h => fun s => match c s with
-                               | inl v => h v s
-                               | inr x => inr x
-                               end
-  }.
+  Global Instance Monad_errS: Monad errS :=
+    { ret  := fun _ x => fun s => inr (s,x)
+      ; bind := fun _ _ m f => fun s => match m s with
+                                  | inl v => inl v
+                                  | inr (s',x) => f x s'
+                                  end
+    }.
 
-Instance State_errS St : MonadState St (errS St) :=
-  {
-    get := fun s => inr (s,s)
-    ; put := fun t s => inr (t, tt)
-  }.
+  Global Instance Exception_errS : MonadExc string errS :=
+    { raise := fun _ v => fun s => inl v
+      ; catch := fun _ c h => fun s => match c s with
+                                 | inl v => h v s
+                                 | inr x => inr x
+                                 end
+    }.
 
+  Global Instance State_errS: MonadState St errS :=
+    {
+      get := fun s => inr (s,s)
+      ; put := fun t s => inr (t, tt)
+    }.
 
-Require Import Vellvm.Error.
+  (* Unwrapping/running monad *)
+  
+  (* Returns value *)
+  Definition evalErrS {A:Type} (c : errS A) (initial : St) : err A :=
+  match c initial with
+  | inl msg => raise msg
+  | inr (s,v) => ret v
+  end.
 
-Definition err2errS {St A: Type}: (err A) -> (errS St A)
-  := fun e => match e with
-           | inl msg => raise msg
-           | inr v => ret v
-           end.
+  (* Returns state *)
+  Definition execErrS {A:Type} (c : errS A) (initial : St) : err St :=
+  match c initial with
+  | inl msg => raise msg
+  | inr (s,v) => ret s
+  end.
 
-Definition option2errS {St A: Type} (msg:string) (o:option A): (errS St A)
-  := match o with
-     | Some v => ret v
-     | None => raise msg
-     end.
+  (* -- lifting [err] -- *)
 
+  Definition err2errS {A: Type}: (err A) -> (errS A)
+    := fun e => match e with
+             | inl msg => raise msg
+             | inr v => ret v
+             end.
+
+  (* -- lifting [option] -- *)
+  
+  Definition option2errS {A: Type} (msg:string) (o:option A): (errS A)
+    := match o with
+       | Some v => ret v
+       | None => raise msg
+       end.
+  
+End withState.
+
+Arguments option2errS {St} {A} (_) (_).
+Arguments err2errS {St} {A} (_).
+Arguments evalErrS {St} {A} (_) (_).
+Arguments execErrS {St} {A} (_) (_).
